existentialsyntax.v
@@ -33,22 +33,22 @@ Definition subst_form_existential   (sigmaterm : ( fin ) -> term ) (s : form_exi
     end.
 
 Variable retract_subst_form : forall   (sigmaterm : ( fin ) -> term ) s, subst_form sigmaterm (inj s) = subst_form_existential sigmaterm s.
-(* 
+
 Definition idSubst_form_existential  (sigmaterm : ( fin ) -> term ) (Eqterm : forall x, sigmaterm x = (var_term ) x) (s : form_existential ) : subst_form_existential sigmaterm s = inj s :=
     match s return subst_form_existential sigmaterm s = inj s with
     | Exist  s0 => congr_Exist_ ((idSubst_form (up_term_term sigmaterm) (upId_term_term (_) Eqterm)) s0)
     end.
-
+(*
 Definition ext_form_existential   (sigmaterm : ( fin ) -> term ) (tauterm : ( fin ) -> term ) (Eqterm : forall x, sigmaterm x = tauterm x) (s : form_existential ) : subst_form_existential sigmaterm s = subst_form_existential tauterm s :=
     match s return subst_form_existential sigmaterm s = subst_form_existential tauterm s with
     | Exist  s0 => congr_Exist_ ((ext_form (up_term_term sigmaterm) (up_term_term tauterm) (upExt_term_term (_) (_) Eqterm)) s0)
     end.
-
+*)
 Definition compSubstSubst_form_existential    (sigmaterm : ( fin ) -> term ) (tauterm : ( fin ) -> term ) (thetaterm : ( fin ) -> term ) (Eqterm : forall x, ((funcomp) (subst_term tauterm) sigmaterm) x = thetaterm x) (s : form_existential ) : subst_form tauterm (subst_form_existential sigmaterm s) = subst_form_existential thetaterm s :=
     match s return subst_form tauterm (subst_form_existential sigmaterm s) = subst_form_existential thetaterm s with
     | Exist  s0 => (eq_trans) (retract_subst_form (_) (Exist (_))) (congr_Exist_ ((compSubstSubst_form (up_term_term sigmaterm) (up_term_term tauterm) (up_term_term thetaterm) (up_subst_subst_term_term (_) (_) (_) Eqterm)) s0))
     end.
-
+(*
 Lemma instId_form_existential  : subst_form_existential (var_term ) = inj .
 Proof. exact ((FunctionalExtensionality.functional_extensionality _ _ ) (fun x => idSubst_form_existential (var_term ) (fun n => eq_refl) ((id) x))). Qed.
 
